src/Init/Data/List/Control.lean
@@ -144,10 +144,10 @@ concatenation of the results.
 @[inline]
 def flatMapM {m : Type u → Type v} [Monad m] {α : Type w} {β : Type u} (f : α → m (List β)) (as : List α) : m (List β) :=
   let rec @[specialize] loop
-    | [],     bs => pure bs.reverse
+    | [],     bs => pure bs.reverse.flatten
     | a :: as, bs => do
       let bs' ← f a
-      loop as (bs' ++ bs)
+      loop as (bs' :: bs)
   loop as []
 
 /--
@@ -284,6 +284,7 @@ instance : ForIn' m (List α) α inferInstance where
 
 -- No separate `ForIn` instance is required because it can be derived from `ForIn'`.
 
+-- We simplify `List.forIn'` to `forIn'`.
 @[simp] theorem forIn'_eq_forIn' [Monad m] : @List.forIn' α β m _ = forIn' := rfl
 
 @[simp] theorem forIn'_nil [Monad m] (f : (a : α) → a ∈ [] → β → m (ForInStep β)) (b : β) : forIn' [] b f = pure b :=
@@ -294,6 +295,9 @@ instance : ForIn' m (List α) α inferInstance where
 
 instance : ForM m (List α) α where
   forM := List.forM
+
+-- We simplify `List.forM` to `forM`.
+@[simp] theorem forM_eq_forM [Monad m] : @List.forM m _ α = forM := rfl
 
 @[simp] theorem forM_nil  [Monad m] (f : α → m PUnit) : forM [] f = pure ⟨⟩ :=
   rfl
